<?xml version="1.0"?>
<rdf:RDF xmlns:rdf="http://www.w3.org/1999/02/22-rdf-syntax-ns#"
  xmlns:foaf="http://xmlns.com/foaf/0.1/"
  xmlns:dct="http://purl.org/dc/terms/"
  xmlns:dc="http://purl.org/dc/elements/1.1/"
  xmlns:rdfs="http://www.w3.org/2000/01/rdf-schema#"
  xmlns:vann="http://purl.org/vocab/vann/"
  xmlns:skos="http://www.w3.org/2004/02/skos/core#"
  xmlns:owl="http://www.w3.org/2002/07/owl#">

  <rdf:Description rdf:about="http://vocab.org/changeset/schema.rdf">
    <rdf:type rdf:resource="http://xmlns.com/foaf/0.1/Document"/>
    <rdf:type rdf:resource="http://purl.org/dc/dcmitype/Text"/>
    <foaf:primaryTopic rdf:resource="http://purl.org/vocab/changeset/schema"/>
    <dct:hasFormat rdf:resource="http://vocab.org/changeset/schema.html"/>
    <dct:hasFormat rdf:resource="http://vocab.org/changeset/schema.json"/>
    <dct:hasFormat rdf:resource="http://vocab.org/changeset/schema.turtle"/>
    <foaf:topic rdf:resource="http://purl.org/vocab/changeset/schema"/>
  </rdf:Description>

  <rdf:Description rdf:about="http://vocab.org/changeset/schema.html">
    <rdf:type rdf:resource="http://purl.org/dc/dcmitype/Text"/>
    <rdf:type rdf:resource="http://xmlns.com/foaf/0.1/Document"/>
    <dc:format>text/html</dc:format>
    <rdfs:label>HTML</rdfs:label>
  </rdf:Description>

  <rdf:Description rdf:about="http://vocab.org/changeset/schema.json">
    <rdf:type rdf:resource="http://purl.org/dc/dcmitype/Text"/>
    <rdf:type rdf:resource="http://xmlns.com/foaf/0.1/Document"/>
    <dc:format>application/json</dc:format>
    <rdfs:label>JSON</rdfs:label>
  </rdf:Description>

  <rdf:Description rdf:about="http://vocab.org/changeset/schema.turtle">
    <rdf:type rdf:resource="http://purl.org/dc/dcmitype/Text"/>
    <rdf:type rdf:resource="http://xmlns.com/foaf/0.1/Document"/>
    <dc:format>text/plain</dc:format>
    <rdfs:label>Turtle</rdfs:label>
  </rdf:Description>

  <rdf:Description rdf:about="http://purl.org/vocab/changeset/schema">
    <rdf:type rdf:resource="http://www.w3.org/2002/07/owl#Ontology"/>
    <dct:date>2006-03-21</dct:date>
    <dct:title xml:lang="en">Changeset</dct:title>
    <rdfs:comment xml:lang="en">
      This vocabulary defines a set of terms for describing changes to resource descriptions.
    </rdfs:comment>
    <rdfs:comment xml:lang="en">
      The vocabulary introduces the notion of a ChangeSet which encapsulates the delta between two versions of a 
      resource description. In this context a resource description is the set of triples that in some way comprise a 
      description of a resource. The delta is represented by two sets of triples: additions and removals. A ChangeSet can be used to 
      modify a resource description by first removing all triples from the description that are in the removals set and
      adding the triples in the additions set.
    </rdfs:comment>
    <dct:identifier>http://purl.org/vocab/changeset/schema-20060321</dct:identifier>
    <dct:isVersionOf rdf:resource="http://purl.org/vocab/changeset/schema#"/>
    <dct:creator>Sam Tunnicliffe</dct:creator>
    <dct:creator rdf:resource="http://iandavis.com/id/me"/>
    <dct:rights>Copyright Â© 2005 Talis Information Ltd.</dct:rights>
    <dct:replaces rdf:resource="http://purl.org/vocab/changeset/schema-20051214"/>
    <vann:preferredNamespaceUri>http://purl.org/vocab/changeset/schema#</vann:preferredNamespaceUri>
    <vann:preferredNamespacePrefix>cs</vann:preferredNamespacePrefix>
    <vann:example rdf:resource="http://vocab.org/changeset/changesets-example-20060321.html"/>
    <vann:example rdf:resource="http://vocab.org/changeset/changesets-example2-20060321.html"/>
    <vann:example rdf:resource="http://vocab.org/changeset/changesets-example3-20060321.html"/>
    <dct:issued>2005-12-14</dct:issued>
    <skos:changeNote rdf:nodeID="mor4e048e385de96"/>
    <skos:changeNote rdf:nodeID="mor4e048e3860d77"/>
    <skos:historyNote rdf:nodeID="mor4e048e385ee36"/>
    <skos:historyNote rdf:nodeID="mor4e048e385fdd6"/>
  </rdf:Description>

  <rdf:Description rdf:about="http://iandavis.com/id/me">
    <rdf:type rdf:resource="http://xmlns.com/foaf/0.1/Person"/>
    <foaf:name>Ian Davis</foaf:name>
  </rdf:Description>

  <rdf:Description rdf:about="http://vocab.org/changeset/changesets-example-20060321.html">
    <dct:title>A Simple ChangeSet</dct:title>
  </rdf:Description>

  <rdf:Description rdf:about="http://vocab.org/changeset/changesets-example2-20060321.html">
    <dct:title>Linked ChangeSets</dct:title>
  </rdf:Description>

  <rdf:Description rdf:about="http://vocab.org/changeset/changesets-example3-20060321.html">
    <dct:title>Implementing Undo With ChangeSets</dct:title>
  </rdf:Description>

  <rdf:Description rdf:nodeID="mor4e048e385de96">
    <rdfs:label xml:lang="en">Improved documentation</rdfs:label>
    <dct:date>2006-03-21</dct:date>
    <dct:creator rdf:resource="http://iandavis.com/id/me"/>
  </rdf:Description>

  <rdf:Description rdf:nodeID="mor4e048e385ee36">
    <rdfs:label xml:lang="en">Introduced statement property</rdfs:label>
    <dct:date>2006-03-21</dct:date>
    <dct:creator rdf:resource="http://iandavis.com/id/me"/>
  </rdf:Description>

  <rdf:Description rdf:nodeID="mor4e048e385fdd6">
    <rdfs:label xml:lang="en">Updated dublin core properties to new namespace</rdfs:label>
    <dct:date>2009-05-18</dct:date>
    <dct:creator rdf:resource="http://iandavis.com/id/me"/>
  </rdf:Description>

  <rdf:Description rdf:nodeID="mor4e048e3860d77">
    <rdfs:label xml:lang="en">Fixed invalid RDF</rdfs:label>
    <dct:date>2006-06-23</dct:date>
    <dct:creator rdf:resource="http://iandavis.com/id/me"/>
  </rdf:Description>

  <rdf:Description rdf:about="http://purl.org/vocab/changeset/schema#statement">
    <rdf:type rdf:resource="http://www.w3.org/2002/07/owl#ObjectProperty"/>
    <rdfs:label xml:lang="en">statement</rdfs:label>
    <skos:definition xml:lang="en">a triple included in this set of changes</skos:definition>
    <rdfs:domain rdf:resource="http://purl.org/vocab/changeset/schema#ChangeSet"/>
    <rdfs:isDefinedBy rdf:resource="http://purl.org/vocab/changeset/schema"/>
    <rdfs:range rdf:resource="http://www.w3.org/1999/02/22-rdf-syntax-ns#Statement"/>
    <dct:issued>2006-03-21</dct:issued>
  </rdf:Description>

  <rdf:Description rdf:about="http://purl.org/vocab/changeset/schema#addition">
    <rdf:type rdf:resource="http://www.w3.org/2002/07/owl#ObjectProperty"/>
    <rdfs:label xml:lang="en">addition</rdfs:label>
    <skos:definition xml:lang="en">a triple to be added to the resource description</skos:definition>
    <rdfs:comment xml:lang="en">
      By convention the subject of the triple being added should be the same as the subjectOfChange
    </rdfs:comment>
    <rdfs:subPropertyOf rdf:resource="http://purl.org/vocab/changeset/schema#statement"/>
    <rdfs:domain rdf:resource="http://purl.org/vocab/changeset/schema#ChangeSet"/>
    <rdfs:isDefinedBy rdf:resource="http://purl.org/vocab/changeset/schema"/>
    <rdfs:range rdf:resource="http://www.w3.org/1999/02/22-rdf-syntax-ns#Statement"/>
    <dct:issued>2005-12-14</dct:issued>
    <skos:changeNote rdf:nodeID="mor4e048e3861d17"/>
    <skos:historyNote rdf:nodeID="mor4e048e3862cb7"/>
    <skos:historyNote rdf:nodeID="mor4e048e3863c57"/>
  </rdf:Description>

  <rdf:Description rdf:nodeID="mor4e048e3861d17">
    <rdf:value>Added definitition and documentation</rdf:value>
    <dct:date>2006-03-21</dct:date>
    <dct:creator>Ian Davis</dct:creator>
  </rdf:Description>

  <rdf:Description rdf:nodeID="mor4e048e3862cb7">
    <rdf:value>Made owl:ObjectProperty</rdf:value>
    <dct:date>2006-03-21</dct:date>
    <dct:creator>Ian Davis</dct:creator>
  </rdf:Description>

  <rdf:Description rdf:nodeID="mor4e048e3863c57">
    <rdf:value>Made a sub-property of statement</rdf:value>
    <dct:date>2006-03-21</dct:date>
    <dct:creator>Ian Davis</dct:creator>
  </rdf:Description>

  <rdf:Description rdf:about="http://purl.org/vocab/changeset/schema#removal">
    <rdf:type rdf:resource="http://www.w3.org/2002/07/owl#ObjectProperty"/>
    <rdfs:label xml:lang="en">removal</rdfs:label>
    <skos:definition xml:lang="en">a triple to be removed from the resource description</skos:definition>
    <rdfs:comment xml:lang="en">
      By convention the subject of the triple being removed should be the same as the subjectOfChange
    </rdfs:comment>
    <rdfs:subPropertyOf rdf:resource="http://purl.org/vocab/changeset/schema#statement"/>
    <rdfs:domain rdf:resource="http://purl.org/vocab/changeset/schema#ChangeSet"/>
    <rdfs:isDefinedBy rdf:resource="http://purl.org/vocab/changeset/schema"/>
    <rdfs:range rdf:resource="http://www.w3.org/1999/02/22-rdf-syntax-ns#Statement"/>
    <dct:issued>2005-12-14</dct:issued>
    <skos:changeNote rdf:nodeID="mor4e048e3864bf7"/>
    <skos:historyNote rdf:nodeID="mor4e048e3865b98"/>
    <skos:historyNote rdf:nodeID="mor4e048e3866b38"/>
  </rdf:Description>

  <rdf:Description rdf:nodeID="mor4e048e3864bf7">
    <rdf:value>Added definitition and documentation</rdf:value>
    <dct:date>2006-03-21</dct:date>
    <dct:creator>Ian Davis</dct:creator>
  </rdf:Description>

  <rdf:Description rdf:nodeID="mor4e048e3865b98">
    <rdf:value>Made owl:ObjectProperty</rdf:value>
    <dct:date>2006-03-21</dct:date>
    <dct:creator>Ian Davis</dct:creator>
  </rdf:Description>

  <rdf:Description rdf:nodeID="mor4e048e3866b38">
    <rdf:value>Made a sub-property of statement</rdf:value>
    <dct:date>2006-03-21</dct:date>
    <dct:creator>Ian Davis</dct:creator>
  </rdf:Description>

  <rdf:Description rdf:about="http://purl.org/vocab/changeset/schema#subjectOfChange">
    <rdf:type rdf:resource="http://www.w3.org/2002/07/owl#ObjectProperty"/>
    <rdfs:label xml:lang="en">subjectOfChange</rdfs:label>
    <skos:definition xml:lang="en">the resource to which this set of changes applies</skos:definition>
    <rdfs:domain rdf:resource="http://purl.org/vocab/changeset/schema#ChangeSet"/>
    <rdfs:isDefinedBy rdf:resource="http://purl.org/vocab/changeset/schema"/>
    <rdfs:range rdf:resource="http://www.w3.org/2000/01/rdf-schema#Resource"/>
    <dct:issued>2005-12-14</dct:issued>
    <skos:changeNote rdf:nodeID="mor4e048e3867ad8"/>
    <skos:historyNote rdf:nodeID="mor4e048e3868a78"/>
  </rdf:Description>

  <rdf:Description rdf:nodeID="mor4e048e3867ad8">
    <rdf:value>Added definitition and documentation</rdf:value>
    <dct:date>2006-03-21</dct:date>
    <dct:creator>Ian Davis</dct:creator>
  </rdf:Description>

  <rdf:Description rdf:nodeID="mor4e048e3868a78">
    <rdf:value>Made owl:ObjectProperty</rdf:value>
    <dct:date>2006-03-21</dct:date>
    <dct:creator>Ian Davis</dct:creator>
  </rdf:Description>

  <rdf:Description rdf:about="http://purl.org/vocab/changeset/schema#precedingChangeSet">
    <rdf:type rdf:resource="http://www.w3.org/2002/07/owl#ObjectProperty"/>
    <rdfs:label xml:lang="en">precedingChangeSet</rdfs:label>
    <skos:definition xml:lang="en">the changeset that immediately precedes this one</skos:definition>
    <rdfs:comment xml:lang="en">
      This property can be used to build a history of changes to a particular resource description. The first
      ChangeSet in the history will have no precedingChangeSet property. Each subsequent ChangeSet added
      to the history references the preceding one resulting in a singly-linked list of changes.  Care must be taken
      not to introduce cycles in the history.
    </rdfs:comment>
    <rdfs:comment xml:lang="en">
      In systems that assume a closed world, the most recent ChangeSet for a particular resource description 
      can be discovered by looking for the ChangeSet that is not the value of a precedingChangeSet property. 
      Conversely, the earliest ChangeSet is the one that is not the subject of a precedingChangeSet property.
    </rdfs:comment>
    <rdfs:domain rdf:resource="http://purl.org/vocab/changeset/schema#ChangeSet"/>
    <rdfs:isDefinedBy rdf:resource="http://purl.org/vocab/changeset/schema"/>
    <rdfs:range rdf:resource="http://purl.org/vocab/changeset/schema#ChangeSet"/>
    <dct:issued>2005-12-14</dct:issued>
    <skos:changeNote rdf:nodeID="mor4e048e3869a19"/>
    <skos:historyNote rdf:nodeID="mor4e048e386a9b9"/>
  </rdf:Description>

  <rdf:Description rdf:nodeID="mor4e048e3869a19">
    <rdf:value>Added definitition and documentation</rdf:value>
    <dct:date>2006-03-21</dct:date>
    <dct:creator>Ian Davis</dct:creator>
  </rdf:Description>

  <rdf:Description rdf:nodeID="mor4e048e386a9b9">
    <rdf:value>Made owl:ObjectProperty</rdf:value>
    <dct:date>2006-03-21</dct:date>
    <dct:creator>Ian Davis</dct:creator>
  </rdf:Description>

  <rdf:Description rdf:about="http://purl.org/vocab/changeset/schema#createdDate">
    <rdf:type rdf:resource="http://www.w3.org/2002/07/owl#DatatypeProperty"/>
    <rdfs:label xml:lang="en">createdDate</rdfs:label>
    <skos:definition xml:lang="en">the date that the changeset was created</skos:definition>
    <rdfs:comment xml:lang="en">
      The date should be in W3CDTF format
    </rdfs:comment>
    <rdfs:domain rdf:resource="http://purl.org/vocab/changeset/schema#ChangeSet"/>
    <rdfs:subPropertyOf rdf:resource="http://purl.org/dc/elements/1.1/date"/>
    <rdfs:isDefinedBy rdf:resource="http://purl.org/vocab/changeset/schema"/>
    <dct:issued>2005-12-14</dct:issued>
    <skos:historyNote rdf:nodeID="mor4e048e386b959"/>
  </rdf:Description>

  <rdf:Description rdf:nodeID="mor4e048e386b959">
    <rdf:value>Made owl:DatatypeProperty</rdf:value>
    <dct:date>2006-03-21</dct:date>
    <dct:creator>Ian Davis</dct:creator>
  </rdf:Description>

  <rdf:Description rdf:about="http://purl.org/vocab/changeset/schema#changeReason">
    <rdf:type rdf:resource="http://www.w3.org/2002/07/owl#DatatypeProperty"/>
    <rdfs:label xml:lang="en">changeReason</rdfs:label>
    <skos:definition xml:lang="en">a  short, human readable description of the purpose for the changeset</skos:definition>
    <rdfs:domain rdf:resource="http://purl.org/vocab/changeset/schema#ChangeSet"/>
    <rdfs:isDefinedBy rdf:resource="http://purl.org/vocab/changeset/schema"/>
    <rdfs:range rdf:resource="http://www.w3.org/2000/01/rdf-schema#Literal"/>
    <dct:issued>2005-12-14</dct:issued>
    <skos:historyNote rdf:nodeID="mor4e048e386c8f9"/>
  </rdf:Description>

  <rdf:Description rdf:nodeID="mor4e048e386c8f9">
    <rdf:value>Made owl:DatatypeProperty</rdf:value>
    <dct:date>2006-03-21</dct:date>
    <dct:creator>Ian Davis</dct:creator>
  </rdf:Description>

  <rdf:Description rdf:about="http://purl.org/vocab/changeset/schema#creatorName">
    <rdf:type rdf:resource="http://www.w3.org/2002/07/owl#DatatypeProperty"/>
    <rdfs:label xml:lang="en">creatorName</rdfs:label>
    <skos:definition xml:lang="en">the name of the entity responsible for creating the changeset</skos:definition>
    <rdfs:domain rdf:resource="http://purl.org/vocab/changeset/schema#ChangeSet"/>
    <rdfs:isDefinedBy rdf:resource="http://purl.org/vocab/changeset/schema"/>
    <rdfs:range rdf:resource="http://www.w3.org/2000/01/rdf-schema#Literal"/>
    <dct:issued>2005-12-14</dct:issued>
    <skos:historyNote rdf:nodeID="mor4e048e386d899"/>
  </rdf:Description>

  <rdf:Description rdf:nodeID="mor4e048e386d899">
    <rdf:value>Made owl:DatatypeProperty</rdf:value>
    <dct:date>2006-03-21</dct:date>
    <dct:creator>Ian Davis</dct:creator>
  </rdf:Description>

  <rdf:Description rdf:about="http://purl.org/vocab/changeset/schema#ChangeSet">
    <rdf:type rdf:resource="http://www.w3.org/2002/07/owl#Class"/>
    <rdfs:label xml:lang="en">ChangeSet</rdfs:label>
    <skos:definition xml:lang="en">The encapsulation of a delta between two versions of a resource description</skos:definition>
    <rdfs:isDefinedBy rdf:resource="http://purl.org/vocab/changeset/schema"/>
    <dct:issued>2005-12-14</dct:issued>
    <skos:changeNote rdf:nodeID="mor4e048e386e83a"/>
    <skos:historyNote rdf:nodeID="mor4e048e386f7da"/>
    <rdfs:subClassOf rdf:nodeID="mor4e048e387077a"/>
  </rdf:Description>

  <rdf:Description rdf:nodeID="mor4e048e386e83a">
    <rdf:value>Improved documentation</rdf:value>
    <dct:date>2006-03-21</dct:date>
    <dct:creator>Ian Davis</dct:creator>
  </rdf:Description>

  <rdf:Description rdf:nodeID="mor4e048e386f7da">
    <rdf:value>Added property cardinality restrictions</rdf:value>
    <dct:date>2006-03-21</dct:date>
    <dct:creator>Ian Davis</dct:creator>
  </rdf:Description>

  <rdf:Description rdf:nodeID="mor4e048e387077a">
    <rdf:type rdf:resource="http://www.w3.org/2002/07/owl#Class"/>
    <owl:intersectionOf rdf:nodeID="mor4e048e387171a"/>
  </rdf:Description>

  <rdf:Description rdf:nodeID="mor4e048e387171a">
    <rdf:first rdf:nodeID="mor4e048e38726bb"/>
    <rdf:rest rdf:nodeID="mor4e048e387365b"/>
  </rdf:Description>

  <rdf:Description rdf:nodeID="mor4e048e38726bb">
    <rdf:type rdf:resource="http://www.w3.org/2002/07/owl#Restriction"/>
    <owl:onProperty rdf:resource="http://purl.org/vocab/changeset/schema#statement"/>
    <owl:minCardinality rdf:datatype="http://www.w3.org/2001/XMLSchema#nonNegativeInteger">1</owl:minCardinality>
  </rdf:Description>

  <rdf:Description rdf:nodeID="mor4e048e387365b">
    <rdf:first rdf:nodeID="mor4e048e38745fb"/>
    <rdf:rest rdf:nodeID="mor4e048e387559b"/>
  </rdf:Description>

  <rdf:Description rdf:nodeID="mor4e048e38745fb">
    <rdf:type rdf:resource="http://www.w3.org/2002/07/owl#Restriction"/>
    <owl:onProperty rdf:resource="http://purl.org/vocab/changeset/schema#previousChangeSet"/>
    <owl:maxCardinality rdf:datatype="http://www.w3.org/2001/XMLSchema#nonNegativeInteger">1</owl:maxCardinality>
  </rdf:Description>

  <rdf:Description rdf:nodeID="mor4e048e387559b">
    <rdf:first rdf:nodeID="mor4e048e387653c"/>
    <rdf:rest rdf:nodeID="mor4e048e38774dc"/>
  </rdf:Description>

  <rdf:Description rdf:nodeID="mor4e048e387653c">
    <rdf:type rdf:resource="http://www.w3.org/2002/07/owl#Restriction"/>
    <owl:onProperty rdf:resource="http://purl.org/vocab/changeset/schema#subjectOfChange"/>
    <owl:maxCardinality rdf:datatype="http://www.w3.org/2001/XMLSchema#nonNegativeInteger">1</owl:maxCardinality>
  </rdf:Description>

  <rdf:Description rdf:nodeID="mor4e048e38774dc">
    <rdf:first rdf:nodeID="mor4e048e387847c"/>
    <rdf:rest rdf:nodeID="mor4e048e387941c"/>
  </rdf:Description>

  <rdf:Description rdf:nodeID="mor4e048e387847c">
    <rdf:type rdf:resource="http://www.w3.org/2002/07/owl#Restriction"/>
    <owl:onProperty rdf:resource="http://purl.org/vocab/changeset/schema#createdDate"/>
    <owl:maxCardinality rdf:datatype="http://www.w3.org/2001/XMLSchema#nonNegativeInteger">1</owl:maxCardinality>
  </rdf:Description>

  <rdf:Description rdf:nodeID="mor4e048e387941c">
    <rdf:first rdf:nodeID="mor4e048e387a3bc"/>
    <rdf:rest rdf:nodeID="mor4e048e387b35d"/>
  </rdf:Description>

  <rdf:Description rdf:nodeID="mor4e048e387a3bc">
    <rdf:type rdf:resource="http://www.w3.org/2002/07/owl#Restriction"/>
    <owl:onProperty rdf:resource="http://purl.org/vocab/changeset/schema#creatorName"/>
    <owl:maxCardinality rdf:datatype="http://www.w3.org/2001/XMLSchema#nonNegativeInteger">1</owl:maxCardinality>
  </rdf:Description>

  <rdf:Description rdf:nodeID="mor4e048e387b35d">
    <rdf:first rdf:nodeID="mor4e048e387c2fd"/>
    <rdf:rest rdf:resource="http://www.w3.org/1999/02/22-rdf-syntax-ns#nil"/>
  </rdf:Description>

  <rdf:Description rdf:nodeID="mor4e048e387c2fd">
    <rdf:type rdf:resource="http://www.w3.org/2002/07/owl#Restriction"/>
    <owl:onProperty rdf:resource="http://purl.org/vocab/changeset/schema#changeReason"/>
    <owl:maxCardinality rdf:datatype="http://www.w3.org/2001/XMLSchema#nonNegativeInteger">1</owl:maxCardinality>
  </rdf:Description>

</rdf:RDF>